generic monadic rules (complex setting)

theories/Relational/GenericRulesComplex.v
@@ -95,7 +95,6 @@ Section RelationalProgramLogicFromRelativeMonad.
       eapply ((actW _ _ _)∙2)=> //; apply (Hm ⦑tt,tt|I⦒).
   Qed.
 
-
     (* move: (rmm_law2 _ _ M12 (W' W) θ _ _ (to_prod f1 f2))=> /= [[H1 H2] H12]. *)
     (* intuition. *)
     (* move: (f_equal (fun h => h m1) H1)=> /= ->. *)
@@ -112,6 +111,122 @@ Section RelationalProgramLogicFromRelativeMonad.
     (* eapply (Spr2 (actW _ _ _))=> //. *)
     (* apply (Hm ⦑tt,tt|I⦒). *)
 
+  (* Program Definition bindWrelStrong *)
+  (*       {Γ A1 A2 B1 B2} *)
+  (*       (wm1 : OrdCat⦅discr (πl Γ); W1 A1⦆) *)
+  (*       (wm2 : OrdCat⦅discr (πr Γ); W2 A2⦆) *)
+  (*       (wmrel : OrdCat⦅discr ⟬Γ⟭; Wrel ⟨A1, A2⟩⦆) *)
+  (*       (wf1 : OrdCat⦅discr (πl Γ × A1); W1 B1⦆) *)
+  (*       (wf2 : OrdCat⦅discr (πr Γ × A2); W2 B2⦆) *)
+  (*       (wfrel : OrdCat⦅discr ⟬extends Γ A1 A2⟭; Wrel ⟨B1, B2⟩⦆) *)
+  (*   : OrdCat⦅discr ⟬Γ⟭; Wrel ⟨B1, B2⟩⦆ := *)
+  (*   ⦑fun γ => (actW (wf1 ∙ ofmap discr (fun a1 => ⟨πl γ, a1⟩)) *)
+  (*                (wf2 ∙ ofmap discr (fun a2 => ⟨πr γ, a2⟩)) *)
+  (*                (wfrel ∙ ofmap discr (fun a12 => extend_point γ (nfst a12) (nsnd a12))) ∙ wmrel)∙1 γ ⦒. *)
+  (* Next Obligation. *)
+  (*   cbv=> ? ?; induction 1 ; apply: rsmc_act_proper; sreflexivity. *)
+  (* Qed. *)
+
+  Notation " X --> Y " := (X -> dfst Y) (at level 99).
+
+  Program Definition to_discr {X Y} (f : X --> Y) : OrdCat⦅discr X; Y⦆ := ⦑f⦒.
+  Next Obligation. move=> ? ?; induction 1; sreflexivity. Qed.
+
+  Definition bindWrelStrong {Γ A1 A2 B1 B2}
+          (wm1 : πl Γ --> W1 A1) (wm2 : πr Γ --> W2 A2)
+          (wmrel : ⟬Γ⟭ --> Wrel ⟨A1, A2⟩)
+          (wf1 : πl Γ × A1 --> W1 B1) (wf2 : πr Γ × A2 --> W2 B2)
+          (wfrel : ⟬extends Γ A1 A2⟭ --> Wrel ⟨B1, B2⟩)
+  : ⟬Γ⟭ --> Wrel ⟨B1, B2⟩ :=
+    fun γ => (actW (to_discr (fun a1 => wf1 ⟨πl γ, a1⟩))
+                (to_discr (fun a2 => wf2 ⟨πr γ, a2⟩))
+                (to_discr (fun '⟨a1,a2⟩ => wfrel (extend_point γ a1 a2))))∙1 (wmrel γ).
+
+  Definition valid (Γ : Rel) A1 A2
+             (c1: πl Γ -> M1 A1) (w1: πl Γ --> W1 A1)
+             (c2:πr Γ -> M2 A2) (w2:πr Γ --> W2 A2)
+             (wrel: ⟬Γ⟭ --> Wrel ⟨A1, A2⟩) : SProp :=
+    ((forall γ1 : πl Γ, (θ1 _)∙1 (c1 γ1) ≤  w1 γ1) s/\
+    (forall γ2 : πr Γ, (θ2 _)∙1 (c2 γ2) ≤ w2 γ2) s/\
+    (forall γ : ⟬Γ⟭, θW∙1 ⟨c1 (πl γ), c2 (πr γ)⟩ ≤ wrel γ)).
+
+  Definition retWrel {A1 A2} : A1 -> A2 --> Wrel ⟨A1,A2⟩ :=
+    fun a1 a2 => (rsmc_return Wrel ⟨A1,A2⟩)∙1 ⟨a1, a2⟩.
+
+  Definition retW {W : unarySpecMonad} {A} : A --> W A := (ord_relmon_unit W A)∙1.
+
+  Lemma ValidRet Γ A1 A2 a1 a2:
+    valid Γ A1 A2  (ret \o a1)  (retW \o a1) (ret \o a2) (retW \o a2)
+          (fun γ => retWrel (a1 (πl γ)) (a2 (πr γ))).
+  Proof.
+    split;[split|]=> γ.
+    - move: (rmm_law1 _ _ _ _ θ1 A1) => /(f_equal (fun f=> f∙1 (a1 γ))) /= ->.
+      sreflexivity.
+    - move: (rmm_law1 _ _ _ _ θ2 A2) => /(f_equal (fun f=> f∙1 (a2 γ))) /= ->.
+      sreflexivity.
+    - move: (@reoc_law1 _ _ _ _ _ _ _ θrc ⟨A1,A2⟩)
+      => /(f_equal (fun f=> f∙1 ⟨a1 (πl γ), a2 (πr γ)⟩)) /= ->.
+      sreflexivity.
+  Qed.
+
+
+  Definition bindWStr {W : unarySpecMonad} {Γ A B}
+             (wm: Γ --> W A) (wf : Γ × A --> W B) : Γ --> W B :=
+    fun γ => (ord_relmon_bind W (to_discr (fun a => wf⟨γ, a⟩)))∙1 (wm γ).
+
+  Lemma ValidBind
+        Γ A1 A2 B1 B2 m1 wm1 m2 wm2 wmrel f1 wf1 f2 wf2 wfrel :
+    valid Γ A1 A2 m1 wm1 m2 wm2 wmrel ->
+    valid (extends Γ A1 A2) B1 B2 f1 wf1 f2 wf2 wfrel ->
+    valid Γ B1 B2
+          (bindStr m1 f1) (bindWStr wm1 wf1)
+          (bindStr m2 f2) (bindWStr wm2 wf2)
+          (bindWrelStrong wm1 wm2 wmrel wf1 wf2 wfrel).
+  Proof.
+    move=> [[Hm1 Hm2] Hm] [[Hf1 Hf2] Hf].
+    split; [split|]=> γ.
+    - move: (rmm_law2 _ _ _ _ θ1 _ _ (fun a => f1 ⟨γ,a⟩))
+      => /(f_equal (fun f=> f∙1 (m1 γ))) /= ->.
+      apply: ordCat_helper; last by apply: Hm1.
+      apply: (ord_relmon_bind_proper W1)=> ? ; apply: Hf1.
+    - move: (rmm_law2 _ _ _ _ θ2 _ _ (fun a=> f2 ⟨γ,a⟩))
+      => /(f_equal (fun f=> f∙1 (m2 γ))) /= ->.
+      apply: ordCat_helper; last by apply: Hm2.
+      apply: (ord_relmon_bind_proper W2)=> ?; apply: Hf2.
+    - move: (reoc_law2 _ _ _ _ _ θrc (to_prod (fun a=> f1 ⟨πl γ,a⟩) (fun a=> f2 ⟨πr γ,a⟩))) => /=.
+      move=> /(f_equal (fun f=> f∙1 ⟨m1 (πl γ),m2 (πr γ)⟩)) /= ->; estransitivity;
+      last (eapply ((actW _ _ _)∙2)=> //; apply (Hm ⦑tt,tt|I⦒)).
+      apply: rsmc_act_proper;
+        [move=> ? ; apply: Hf1| move=> ?; apply: Hf2|].
+      move=> [? ?] /=; set γ' := extend_point _ _ _; apply: (Hf γ').
+  Qed.
+
+  Notation "x ⩿ y" := (pointwise_srelation _ (@extract_ord _) x y) (at level 70).
+
+  Lemma ValidWeaken
+             Γ A1 A2 m1 wm1 wm1' m2 wm2 wm2' wmrel wmrel':
+    valid Γ A1 A2 m1 wm1 m2 wm2 wmrel ->
+    wm1 ⩿ wm1' -> wm2 ⩿ wm2' -> wmrel ⩿ wmrel' ->
+    valid Γ A1 A2 m1 wm1' m2 wm2' wmrel'.
+  Proof.
+    move=> [[H1 H2] H] Hle1 Hle2 Hle; split; [split|] => ?; estransitivity.
+    apply: H1. apply: Hle1.
+    apply: H2. apply: Hle2.
+    apply: H. apply: Hle.
+  Qed.
+
+  Lemma ValidSubst Γ Δ A1 A2 m1 wm1 m2 wm2 wmrel (σ: Δ R==> Γ) :
+    valid Γ A1 A2 m1 wm1 m2 wm2 wmrel ->
+    valid Δ A1 A2
+          (m1 \o πl σ) (wm1 \o πl σ)
+          (m2 \o πr σ) (wm2 \o πr σ)
+          (wmrel \o applyRel _ _ σ).
+  Proof.
+    move=> [[H1 H2] H]; split; [split|]=> γ.
+    apply: H1.
+    apply: H2.
+    set γ' := (σ @R γ); exact: (H γ').
+  Qed.
 
   (* Definition bindStrongRSM {Γ A1 A2 B1 B2} *)
   (*            (wm1 : πl Γ -> W1 A1) *)
